\documentclass[12pt]{article}
\usepackage[paper=a4paper,left=25mm,right=25mm,top=25mm,bottom=25mm]{geometry}
\usepackage[english]{babel}
\usepackage[utf8]{inputenc}
\usepackage[pdftex]{graphicx}
\usepackage{color}
\usepackage{amssymb}
\usepackage{amsthm}
\usepackage{hyperref}
\usepackage{enumitem}
\usepackage{pdfpages}
\usepackage{hyperref}


\linespread{1.25}

\begin{document}
\begin{titlepage}
\includegraphics[height=20mm]{../images/uzh_logo}\\

\begin{flushleft}

\vspace{2cm}

{\Large Introduction to Artificial Intelligence\\Exercise Sheet 8}\\

\vspace{4cm}

\textbf{Laurin van den Bergh, 16-744-401\\Yufeng Xiao, 19-763-663\\Nora Beringer, 19-734-227}\\

\vspace{2cm}

Universität Zürich\\
Institut für Informatik

\vfill Due: May 04, 2022

\vspace{3cm}


\end{flushleft}
\end{titlepage}

\newpage

\section*{Exercise 8.1}

\textbf{(a)} $\mathbb{P}$(c = fake) = 1$\div n$\\
\textbf{(b)} We assume that the event is dependent of getting k heads and the fake coin.\\
$\mathbb{P}$(c = fake $\mid$ k heads) = $\frac{\mathbb{P}(k heads \mid c = fake) * \mathbb{P}(c = fake)}{\mathbb{P}(k heads)}$ = $\frac{\frac{1}{n}}{\frac{1}{n} + \frac{n-1}{n} * (\frac{1}{2})^{k}}$\\
\textbf{(c)} $\mathbb{P}(c = normal \mid k heads)$ = $\frac{\mathbb{P}(k heads \mid c = normal) * \mathbb{P}(c = normal)}{\mathbb{P}(k heads)}$ = $\frac{(\frac{1}{2})^{k} * \frac{n-1}{n}}{\frac{1}{n} * 1 + \frac{n-1}{n} * (\frac{1}{2})^{k}}$ = $\frac{(\frac{1}{2})^{k} * (n-1)}{1+(\frac{1}{2})^{k}*(n-1)}$ = $\frac{1}{1+\frac{1}{(\frac{1}{2})^{k}*(n-1)}}$

\section*{Exercise 8.2}

\textbf{(a)} $\mathbb{P}$(positive result $\mid$ Test A = positive) = $\frac{\mathbb{P}(Test A = positive  \mid positive result) * \mathbb{P}(positive result)}{\mathbb{P}(Test A = positive)}$ = $\frac{0.95*0.01}{0.01*0.95 + 0.99*0.01}$ = $\frac{0.095}{0.095+0.099}$ = 0.0876\\
$\mathbb{P}$(positive result $\mid$ Test B = positive) = $\frac{\mathbb{P}(Test B = positive \mid positive)* \mathbb{P}(positive)}{\mathbb{P}(Test B = positive)}$ = $\frac{0.9*0.01}{0.9*0.01+0.99*0.05}$ = $\frac{0.009}{0.009+0.0495}$ = 0.155\\
\textbf{(b)} $\mathbb{P}$(positive result $\mid$ Test A = positive) = $\frac{\mathbb{P}(Test A = positive  \mid positive result) * \mathbb{P}(positive result)}{\mathbb{P}(Test A = positive)}$ = $\frac{0.95*0.3}{0.3*0.95 + 0.7*0.1}$ = 0.802\\
$\mathbb{P}$(positive result $\mid$ Test B = positive) = $\frac{\mathbb{P}(Test B = positive \mid positive)* \mathbb{P}(positive)}{\mathbb{P}(Test B = positive)}$ = $\frac{0.9*0.3}{0.9*0.3+0.7*0.05}$ = 0.885\\

\section*{Exercise 8.3}

\textbf{(a)}\\
\textbf{(b)}\\
\textbf{(c)}



\end{document}